formal/tlaplus/deploy_recovery/ProtocolDeployIngress.tla
@@ -3,12 +3,23 @@ EXTENDS FiniteSets, Integers
 
 CONSTANT
     \* @type: Bool;
-    EnforceProtocolIngress
+    EnforceProtocolIngress,
+    \* @type: Bool;
+    EnforceBlockWindow
 
-ASSUME EnforceProtocolIngress \in BOOLEAN
+ASSUME /\ EnforceProtocolIngress \in BOOLEAN
+       /\ EnforceBlockWindow \in BOOLEAN
 
 Protocols == {5, 6}
 Kinds == {"legacy", "envelope"}
+Ids == 0..1
+MaxTip == 2
+Lifespan == 1
+
+ValidAfter(id) == 0
+
+WindowOpen(id, observedTip) ==
+    ValidAfter(id) > observedTip - Lifespan
 
 VARIABLES
     \* @type: Int;
@@ -18,47 +29,70 @@ VARIABLES
     \* @type: Set(Int);
     envelopePool,
     \* @type: Int;
-    nextId
+    nextId,
+    \* @type: Int;
+    tip,
+    \* @type: (Int -> Int);
+    admissionTip
 
-vars == <<protocol, legacyPool, envelopePool, nextId>>
+vars == <<protocol, legacyPool, envelopePool, nextId, tip, admissionTip>>
 
 Init ==
     /\ protocol \in Protocols
     /\ legacyPool = {}
     /\ envelopePool = {}
     /\ nextId = 0
+    /\ tip = 0
+    /\ admissionTip = [id \in Ids |-> -1]
 
 LegacyAuthorized == protocol < 6
 EnvelopeAuthorized == protocol >= 6
 
 SubmitLegacy ==
-    /\ legacyPool' =
-        IF EnforceProtocolIngress /\ ~LegacyAuthorized
-        THEN legacyPool
-        ELSE legacyPool \union {nextId}
+    /\ nextId \in Ids
+    /\ LET accepted ==
+            (~EnforceProtocolIngress \/ LegacyAuthorized)
+            /\ (~EnforceBlockWindow \/ WindowOpen(nextId, tip))
+       IN /\ legacyPool' = IF accepted THEN legacyPool \union {nextId} ELSE legacyPool
+          /\ admissionTip' = IF accepted
+                              THEN [admissionTip EXCEPT ![nextId] = tip]
+                              ELSE admissionTip
     /\ nextId' = nextId + 1
-    /\ UNCHANGED <<protocol, envelopePool>>
+    /\ UNCHANGED <<protocol, envelopePool, tip>>
 
 SubmitEnvelope ==
-    /\ envelopePool' =
-        IF EnforceProtocolIngress /\ ~EnvelopeAuthorized
-        THEN envelopePool
-        ELSE envelopePool \union {nextId}
+    /\ nextId \in Ids
+    /\ LET accepted ==
+            (~EnforceProtocolIngress \/ EnvelopeAuthorized)
+            /\ (~EnforceBlockWindow \/ WindowOpen(nextId, tip))
+       IN /\ envelopePool' = IF accepted THEN envelopePool \union {nextId} ELSE envelopePool
+          /\ admissionTip' = IF accepted
+                              THEN [admissionTip EXCEPT ![nextId] = tip]
+                              ELSE admissionTip
     /\ nextId' = nextId + 1
-    /\ UNCHANGED <<protocol, legacyPool>>
+    /\ UNCHANGED <<protocol, legacyPool, tip>>
 
-Next == nextId < 2 /\ (SubmitLegacy \/ SubmitEnvelope)
+AdvanceTip ==
+    /\ tip < MaxTip
+    /\ tip' = tip + 1
+    /\ UNCHANGED <<protocol, legacyPool, envelopePool, nextId, admissionTip>>
+
+Next == SubmitLegacy \/ SubmitEnvelope \/ AdvanceTip
 
 Spec == Init /\ [][Next]_vars
 
 TypeOK ==
     /\ protocol \in Protocols
-    /\ legacyPool \subseteq 0..nextId
-    /\ envelopePool \subseteq 0..nextId
-    /\ nextId \in Nat
+    /\ legacyPool \subseteq Ids
+    /\ envelopePool \subseteq Ids
+    /\ nextId \in 0..Cardinality(Ids)
+    /\ tip \in 0..MaxTip
+    /\ admissionTip \in [Ids -> -1..MaxTip]
 
 V6HasNoLegacyPool == protocol >= 6 => legacyPool = {}
 PreV6HasNoEnvelopePool == protocol < 6 => envelopePool = {}
 PoolDomainsAreDisjoint == legacyPool \intersect envelopePool = {}
+IngressWindowSound ==
+    \A id \in legacyPool \union envelopePool : WindowOpen(id, admissionTip[id])
 
 =============================================================================
